G2 equivalence

src/Hacspec/Curve/EquivToBedrock.v
@@ -16,6 +16,7 @@ From Coqprime Require Import GZnZ.
 Require Import Hacspec.Curve.Bls.
 Require Import Hacspec.Curve.BlsProof.
 Require Import Field.
+Require Import Crypto.Util.ZUtil.Tactics.PullPush.Modulo.
 
 
 Local Open Scope Z_scope.
@@ -96,7 +97,7 @@ Definition fc_field := ZpZfc m blsprime.
 Lemma three_small : 3 < m.
 Proof. reflexivity. Qed.
 
-Definition char_ge_3 := (Char_geq_p m 3%positive three_small).
+Definition char_ge_3 := (Char_geq_p m (N.succ_pos N.two) three_small).
 
 Lemma fp_dec: DecidableRel (@eq (znz m)).
 Proof. unfold Decidable. intros [x Hx] [y Hy]. generalize (Z.eqb_eq x y). intros H. destruct (x =? y) eqn:E.
@@ -164,34 +165,25 @@ Lemma val_eq: forall x H, val m (mkznz m x H) = x.
 Proof. intros. reflexivity. Qed.
 
 Lemma add_elim_mod: forall x y, x mod m +' y mod m = x +' y.
-Proof. intros. unfold my_add. symmetry. apply Zplus_mod. Qed.
+Proof. intros. unfold my_add. pull_Zmod. reflexivity. Qed.
 
 Lemma mul_elim_mod: forall x y, (x mod m) *' (y mod m) = x *' y.
-Proof. intros. unfold my_mul. symmetry. apply Z.mul_mod. unfold m. congruence. Qed.
+Proof. intros. unfold my_mul. pull_Zmod. reflexivity. Qed.
 
 Lemma sub_elim_mod: forall x y, x mod m -' y mod m = x -' y.
-Proof. intros. unfold my_sub. symmetry. apply Zminus_mod. Qed.
+Proof. intros. unfold my_sub. pull_Zmod. reflexivity. Qed.
 
 Ltac znz_toz_arith := unfold fp_a, fp_3_b; repeat (try rewrite add_eq; try rewrite mul_eq; try rewrite sub_eq; try rewrite val_eq; try rewrite add_elim_mod; try rewrite mul_elim_mod; try rewrite sub_elim_mod); rewrite <- a_small, <- three_b_small.
 Ltac znz_toz_arith_h H := unfold fp_a, fp_3_b in H; repeat (try rewrite add_eq in H; try rewrite mul_eq in H; try rewrite sub_eq in H; try rewrite val_eq in H; try rewrite add_elim_mod in H; try rewrite mul_elim_mod in H; try rewrite sub_elim_mod in H); rewrite <- a_small, <- three_b_small in H.
+Ltac rememberp X1 X2 Y1 Y2 Z1 Z2 := remember (evfrom X1) as x1; remember (evfrom X2) as x2; remember (evfrom Y1) as y1; remember (evfrom Y2) as y2; remember (evfrom Z1) as z1; remember (evfrom Z2) as z2.
 
 (* Equivalence between galina and fiat with eq relation*)
 Lemma galina_fiat_crypto_equiv : forall X1 X2 Y1 Y2 Z1 Z2 outx outy outz on_curve1 on_curve2 except, 
     (BLS12_add_Gallina_spec X1 Y1 Z1 X2 Y2 Z2 outx outy outz <-> 
     (evfrom outx, evfrom outy, evfrom outz) = pair_val (proj1_sig (fc_proj_add (to_fc_point_from_mont X1 Y1 Z1 on_curve1) (to_fc_point_from_mont X2 Y2 Z2 on_curve2) except))).
-Proof. split.
-    - unfold BLS12_add_Gallina_spec. unfold MontgomeryCurveSpecs.BLS12_add_Gallina_spec. intros H. apply pair_equal_spec in H. destruct H as [H H3]. apply pair_equal_spec in H. destruct H as [H1 H2].
-    apply pair_equal_spec. split.
-        + apply pair_equal_spec. split.
-            * znz_toz_arith. rewrite H1. reflexivity.
-            * znz_toz_arith. rewrite H2. reflexivity.
-        + znz_toz_arith. rewrite H3. reflexivity.
-    - intros H. apply pair_equal_spec in H. destruct H as [H H3]. apply pair_equal_spec in H. destruct H as [H1 H2].
-    apply pair_equal_spec. split.
-        + apply pair_equal_spec. split.
-         * rewrite H1. znz_toz_arith.  reflexivity.
-         * rewrite H2. znz_toz_arith. reflexivity.
-        + rewrite H3. znz_toz_arith. reflexivity.
+Proof. assert (forall A (x y z: A), y = z -> (x = y <-> x = z)). {  intros. rewrite H. reflexivity. } 
+    intros. apply H. unfold pair_val, fc_proj_add, proj1_sig, to_fc_point_from_mont, to_fc_point.
+    rememberp X1 X2 Y1 Y2 Z1 Z2. znz_toz_arith. reflexivity.
 Qed.
 
 
@@ -205,20 +197,11 @@ Lemma galina_fiat_crypto_equiv' : forall X1 Y1 Z1 X2 Y2 Z2 outx outy outz on_cur
     (BLS12_add_Gallina_spec X1 Y1 Z1 X2 Y2 Z2 outx outy outz -> 
     fc_proj_eq (to_fc_point_from_mont outx outy outz on_curve_out)  (fc_proj_add (to_fc_point_from_mont X1 Y1 Z1 on_curve1) (to_fc_point_from_mont X2 Y2 Z2 on_curve2) except)).
 Proof. intros. rewrite (galina_fiat_crypto_equiv _ _ _ _ _ _ _ _ _ on_curve1 on_curve2 except) in H. 
-     apply fc_proj_eq_sig.  apply pair_equal_spec in H. destruct H as [H H3]. apply pair_equal_spec in H. destruct H as [H1 H2].
-      apply pair_equal_spec.
-      remember (evfrom X1) as x1.
-        remember (evfrom X2) as x2.
-        remember (evfrom Y1) as y1.
-        remember (evfrom Y2) as y2.
-        remember (evfrom Z1) as z1.
-        remember (evfrom Z2) as z2.
-        split; [apply pair_equal_spec; split |].
-        + destruct H2, H3. znz_toz_arith_h H1. rewrite H1. apply zirr. znz_toz_arith. unfold "-'". rewrite Zmod_mod. reflexivity.
-        + destruct H1, H3. znz_toz_arith_h H2. rewrite H2. apply zirr. znz_toz_arith. unfold "+'". rewrite Zmod_mod. reflexivity.
-        + destruct H1, H2. znz_toz_arith_h H3. rewrite H3. apply zirr. znz_toz_arith. unfold "+'". rewrite Zmod_mod. reflexivity.
+    apply fc_proj_eq_sig. unfold to_fc_point_from_mont, to_fc_point, fc_proj_add, proj1_sig.
+    apply pair_equal_spec in H.     rememberp X1 X2 Y1 Y2 Z1 Z2. 
+    destruct H as [H ->]. apply pair_equal_spec in H. destruct H as [-> ->].
+    apply pair_equal_spec. split; [apply pair_equal_spec; split |]; apply zirr; znz_toz_arith; unfold "-'", "+'"; rewrite Zmod_mod; reflexivity.
 Qed.
-
 
 Definition galina_spec_from_fc_point (p1 p2 pout : fc_proj_point) := 
     let '(x1, y1, z1) := pair_val (proj1_sig p1) in
@@ -252,9 +235,7 @@ Lemma galina_fiat_crypto_equiv'' : forall p1 p2 pout except,
     fc_proj_eq pout (fc_proj_add p1 p2 except) ->
     exists pout', fc_proj_eq pout pout' /\ galina_spec_from_fc_point p1 p2 pout'.
 Proof. intros. exists (fc_proj_add p1 p2 except).
-    split.
-    - apply H.
-    - unfold galina_spec_from_fc_point, BLS12_add_Gallina_spec, MontgomeryCurveSpecs.BLS12_add_Gallina_spec.
+    split; [apply H|]. unfold galina_spec_from_fc_point, BLS12_add_Gallina_spec, MontgomeryCurveSpecs.BLS12_add_Gallina_spec.
     destruct p1 as [[[]]]. destruct p2 as [[[]]]. unfold fc_proj_add, proj1_sig, pair_val. 
     repeat rewrite eval_encodemod_val. znz_toz_arith. rewrite eval_three_b_list. rewrite eval_a_list. reflexivity.
 Qed.
@@ -265,28 +246,12 @@ Definition to_hacspec_point (X1 Y1 Z1 : list Z) on_curve : g1 := g1_from_fc (to_
 Add Field hs_fp_field: fp_field_theory.
 
 Lemma preserves_on_curve : forall p, g1_on_curve (g1_from_fc p).
-Proof. intros p.  unfold g1_on_curve. destruct p. destruct x.
-- destruct p. cbn. rewrite y.  field.
-- cbn. destruct u. trivial.
+Proof. intros [[[] | []]]; cbn; auto.  rewrite y. field.
 Qed.
 
 Lemma g1_fc_eq: forall x y :fc_aff_point, g1_from_fc x ?=? g1_from_fc y <-> fc_aff_eq x y.
 Proof.
-    intros [[[] | []]] [[[] | []]]; unfold "?=?", fc_aff_eq; cbn.
-    - split. 
-        + intros []. apply H0.
-        + intros. split. 
-            * reflexivity.
-            * apply H.
-    - split. 
-        + intros []. discriminate H.
-        + intros [].
-    - split.
-        + intros c. discriminate c.
-        + intros [].
-    - split.
-        + trivial.
-        + reflexivity.
+    intros [[[] | []]] [[[] | []]]; unfold "?=?", fc_aff_eq; cbn; split; intros H; inversion H; auto; discriminate.
 Qed.
 
 Lemma same_field_opp : forall x, Lib.nat_mod_neg x = opp m x.
@@ -298,29 +263,21 @@ Qed.
 
 
 Lemma same_fc_add: forall x y, fc_aff_eq (g1_fc_add x y) (fc_aff_add x y).
-Proof. intros [[[] | []]] [[[] | []]]; unfold g1_fc_add; unfold fc_aff_add; unfold fc_aff_eq; cbn.
-- unfold dec. do 2 rewrite dec_same. rewrite same_field_opp. destruct (fp_dec f f1); destruct (fp_dec f2 (opp m f0));
-    try trivial; split;  reflexivity.
-- split; reflexivity. 
-- split; reflexivity.
-- trivial.
+Proof. intros [[[] | []]] [[[] | []]]; unfold g1_fc_add; unfold fc_aff_add; unfold fc_aff_eq; cbn; auto.
+ unfold dec. do 2 rewrite dec_same. rewrite same_field_opp. destruct (fp_dec f f1); destruct (fp_dec f2 (opp m f0));
+    try trivial; split; reflexivity.
 Qed.
 
 Lemma fc_aff_eq_refl: forall x, fc_aff_eq x x.
-Proof. intros [[[]| []]]; cbn.
-- split; reflexivity.
-- trivial.
+Proof. intros [[[]| []]]; cbn; auto.
 Qed.
 
 Lemma fc_aff_eq_symm: forall x y, fc_aff_eq x y -> fc_aff_eq y x.
-Proof. intros [[[] | []]] [[[] | []]]; unfold fc_aff_eq; cbn; intros [].
-    - rewrite H. rewrite H0. split; reflexivity.
-    - trivial.
+Proof. intros [[[] | []]] [[[] | []]]; unfold fc_aff_eq; cbn; intros []; auto.
 Qed.
 
 Lemma fc_aff_eq_trans: forall x y z, fc_aff_eq x y -> fc_aff_eq y z -> fc_aff_eq x z.
-Proof.  intros [[[] | []]] [[[] | []]] [[[] | []]]; unfold fc_aff_eq; cbn; intros [] []; try trivial.
-    - rewrite H. rewrite H1. rewrite H0. rewrite H2. split; reflexivity.
+Proof.  intros [[[] | []]] [[[] | []]] [[[] | []]]; unfold fc_aff_eq; cbn; intros [] []; subst; auto.
 Qed. 
 
 Add Relation fc_aff_point fc_aff_eq
@@ -378,3 +335,192 @@ Proof.
     apply galina_fiat_crypto_equiv'' in H0. apply H0. 
 Qed.
 
+(** G2 Equivalence section **)
+Require Import Crypto.Arithmetic.Partition.
+Require Import Theory.Fields.QuadraticFieldExtensions.
+Require Import Crypto.Algebra.Hierarchy.
+
+Local Notation br := (4 mod m).
+Local Notation bi := (4 mod m).
+
+Local Notation three_br := (3 * br mod m).
+Local Notation three_bi := (3 * bi mod m).
+
+Definition BLS12_G2_add_Gallina_spec X1 Y1 Z1 X2 Y2 Z2 outx outy outz :=
+    @BLS12_G2_add_Gallina_spec m bw n m' 0 0 three_br three_bi X1 Y1 Z1 X2 Y2 Z2 outx outy outz.
+
+Local Infix "*p2'" := (my_mulFp2 m) (at level 40).
+Local Infix "+p2'" := (my_addFp2 m) (at level 50).
+Local Infix "-p2'" := (my_subFp2 m) (at level 50).
+
+Local Infix "*m2" := (mulp2 m) (at level 40).
+Local Infix "+m2" := (addp2 m) (at level 50).
+Local Infix "-m2" := (subp2 m) (at level 50).
+
+
+Local Notation Fp2 := (znz m * znz m)%type.
+Definition fp2_a := zerop2 m.
+Definition fp2_b := (fp_b, fp_b).
+
+Lemma m_odd: 2 < m.
+Proof. reflexivity. Qed.
+
+Lemma m_mod3: m mod 4 =? 3 = true.
+Proof. reflexivity. Qed.
+
+Check (@FFp2 m) blsprime m_odd m_mod3.
+Local Notation FFp2 := ((@FFp2 m) blsprime m_odd m_mod3).
+Add Field fp2_field : FFp2.
+
+(*field_theory (zerop2 m) (onep2 m) (addp2 m) (mulp2 m)
+(subp2 m) (oppp2 m) (divp2 m) (invp2 m) (@eq Fp2).*)
+Check (Fp2fc m blsprime m_odd m_mod3).
+Definition fp2_fc_field := (Fp2fc m blsprime m_odd m_mod3).
+Definition fp2_char_ge_3 := Char_Fp2_geq_p m blsprime 3 three_small.
+Definition fp2_char_ge_21 := Char_Fp2_geq_p m blsprime 21 twenty1_small.
+
+Lemma fc_fp2_dec : DecidableRel (@eq (Fp2)).
+Proof. unfold Decidable. apply eq_dec_Fp2. Qed.
+
+Local Notation fp2_3_b := (fp2_b +m2 fp2_b +m2 fp2_b).
+
+Lemma mul_zero_r: forall x, x *m (zero m) = zero m.
+Proof. intros []. unfold "*m". cbn. rewrite Z.mul_0_r. reflexivity. 
+Qed.
+
+Lemma mul_zero_l: forall x, (zero m) *m x = zero m.
+Proof. intros [].  reflexivity. 
+Qed.
+
+Lemma mulp2_zero: forall p, p *m2 (zerop2 m) = (zerop2 m).
+Proof. intros []. unfold zerop2, mulp2, fst, snd. repeat rewrite mul_zero_r. reflexivity. 
+Qed. 
+
+Lemma fp2_discriminant_nonzero: id(((mkznz m _ (modz m 4), zero m) *m2 fp2_a *m2 fp2_a *m2 fp2_a +m2 (mkznz m _ (modz m 27), zero m) *m2 fp2_b *m2 fp2_b) <> (zerop2 m)).
+Proof.  unfold id, fp2_a, fp_a, fp2_b, fp_b, zerop2, addp2, mulp2, fst, snd.  
+    intros c. apply pair_equal_spec in c. destruct c.  repeat rewrite mul_zero_r in H0. discriminate H0.
+Qed.
+
+Local Notation fc_proj_p2_point := (@Projective.point Fp2 eq (zerop2 m) (addp2 m) (mulp2 m) fp2_a fp2_b).
+Check (@Projective.add Fp2 eq (zerop2 m) (onep2 m) (oppp2 m) (addp2 m) (subp2 m) (mulp2 m) (invp2 m) (divp2 m) fp2_a fp2_b fp2_fc_field fp2_char_ge_3 fc_fp2_dec fp2_3_b (eq_refl) fp2_discriminant_nonzero fp2_char_ge_21).
+Local Notation fc_proj_p2_add :=  (@Projective.add Fp2 eq (zerop2 m) (onep2 m) (oppp2 m) (addp2 m) (subp2 m) (mulp2 m) (invp2 m) (divp2 m) fp2_a fp2_b fp2_fc_field fp2_char_ge_3 fc_fp2_dec fp2_3_b (eq_refl) fp2_discriminant_nonzero fp2_char_ge_21).
+Local Notation fc_proj_p2_eq := (@Projective.eq Fp2 eq (zerop2 m) (addp2 m) (mulp2 m) fp2_a fp2_b fc_fp2_dec).
+
+
+Definition On_Curve_p2 (X1 Y1 Z1 : Fp2) := (Y1 *m2 Y1 *m2 Z1) = (X1 *m2 (X1 *m2 X1) +m2 fp2_a *m2 X1 *m2 (Z1 *m2 Z1) +m2 fp2_b *m2 (Z1 *m2 (Z1 *m2 Z1))) /\ (Z1 = zerop2 m -> Y1 <> zerop2 m).
+
+Program Definition to_fc_p2_point (X1 Y1 Z1 : Fp2) (on_curve : On_Curve_p2 X1 Y1 Z1) : fc_proj_p2_point := 
+     (X1, Y1, Z1).
+
+Local Notation evfrom_pair := (evfrom_pair m bw n m').
+
+Definition Fp2_from_Z_Z (x: Z*Z) : Fp2 := (mkznz _ _ (modz m (fst x)), mkznz _ _ (modz m (snd x))).
+
+Definition to_fc_p2_point_from_mont X1 Y1 Z1 on_curve := to_fc_p2_point (Fp2_from_Z_Z (evfrom_pair X1)) (Fp2_from_Z_Z (evfrom_pair Y1)) (Fp2_from_Z_Z (evfrom_pair Z1)) on_curve.
+
+Definition valp2 x := (val m (fst x), val m (snd x)).
+
+Definition pair_p2_val (x: Fp2*Fp2*Fp2) := let '(x, y, z) := x in (valp2 x, valp2 y, valp2 z).
+
+Definition pair_mod x := (fst x mod m, snd x mod m).
+
+
+Add Field fc_field : (FZpZ m blsprime).
+
+Lemma Quad_neg_one: (Quad_non_res m = opp m (one m)).
+Proof. reflexivity. Qed.
+
+Lemma addp2_eq: forall x y : Fp2, valp2 (x +m2 y) = (valp2 x) +p2' (valp2 y).
+Proof. intros. reflexivity. Qed.
+
+Lemma mulp2_eq: forall x y : Fp2, valp2 (x *m2 y) = (valp2 x) *p2' (valp2 y).
+Proof. intros [] []. unfold "*m2", "*p2'". rewrite Quad_neg_one. cbn. 
+    assert (z *m z1 +m (opp m (one m) *m z0) *m z2 = z *m z1 -m z0 *m z2). { field. }
+    rewrite H. unfold valp2. cbn. pull_Zmod. reflexivity.
+Qed.
+
+Lemma subp2_eq: forall x y : Fp2, valp2 (x -m2 y) = (valp2 x) -p2' (valp2 y).
+Proof. intros. reflexivity. Qed.
+
+Lemma valp2_eq: forall x, valp2 (Fp2_from_Z_Z x) = pair_mod x.
+Proof. reflexivity. Qed.
+
+Lemma addp2_elim_mod: forall x y, pair_mod x +p2' pair_mod y = x +p2' y.
+Proof. intros [] []. unfold "+p2'". cbn. pull_Zmod. reflexivity.
+Qed.
+
+Lemma mulp2_elim_mod: forall x y, pair_mod x *p2' pair_mod y = x *p2' y.
+Proof. intros [] []. unfold "*p2'". cbn. push_Zmod. reflexivity. 
+Qed.
+
+Lemma subp2_elim_mod: forall x y, pair_mod x -p2' pair_mod y = x -p2' y.
+Proof. intros [] []. unfold "-p2'". cbn. pull_Zmod. reflexivity.
+Qed. 
+
+Lemma three_bp2_eq: (eval (three_br_list bw n three_bi), eval (three_bi_list bw n three_bi)) = valp2 fp2_3_b.
+Proof. reflexivity. Qed.
+
+Lemma ap2_eq: (eval (ar_list bw n 0), eval (ai_list bw n 0)) = valp2 fp2_a.
+Proof. reflexivity. Qed.
+
+Ltac znz2_to_z2_arith := rewrite three_bp2_eq; rewrite ap2_eq; repeat (try rewrite addp2_eq; try rewrite mulp2_eq; try rewrite subp2_eq; try rewrite valp2_eq; try rewrite addp2_elim_mod; try rewrite mulp2_elim_mod; try rewrite subp2_elim_mod).
+Ltac rememberp2 X1 X2 Y1 Y2 Z1 Z2 := remember (evfrom_pair X1) as x1; remember (evfrom_pair X2) as x2; remember (evfrom_pair Y1) as y1; remember (evfrom_pair Y2) as y2; remember (evfrom_pair Z1) as z1; remember (evfrom_pair Z2) as z2.  
+
+Lemma galina_fiat_crypto_p2_equiv : forall X1 X2 Y1 Y2 Z1 Z2 outx outy outz on_curve1 on_curve2 except, 
+    (BLS12_G2_add_Gallina_spec X1 Y1 Z1 X2 Y2 Z2 outx outy outz <-> 
+    (evfrom_pair outx, evfrom_pair outy, evfrom_pair outz) = pair_p2_val (proj1_sig (fc_proj_p2_add (to_fc_p2_point_from_mont X1 Y1 Z1 on_curve1) (to_fc_p2_point_from_mont X2 Y2 Z2 on_curve2) except))).
+Proof. assert (forall A (x y z: A), y = z -> (x = y <-> x = z)). {  intros. rewrite H. reflexivity. }
+    intros. unfold BLS12_G2_add_Gallina_spec, MontgomeryCurveSpecs.BLS12_G2_add_Gallina_spec, to_fc_p2_point_from_mont.
+    apply H. unfold pair_p2_val, fc_proj_p2_add, proj1_sig, to_fc_p2_point. 
+    rememberp2 X1 X2 Y1 Y2 Z1 Z2. znz2_to_z2_arith. reflexivity.
+Qed.
+
+Lemma fc_proj_p2_eq_sig: forall x y, proj1_sig x = proj1_sig y -> fc_proj_p2_eq x y.
+Proof. intros [[[]]] [[[]]] H. cbn. inversion H. destruct (dec (p4 = zerop2 m))eqn:E1; [apply e |].
+    split ; reflexivity.
+Qed. 
+
+Lemma p2_backandforth: forall p, Fp2_from_Z_Z (valp2 p) = p.
+Proof. intros [[][]]. apply pair_equal_spec. split; apply zirr; cbn; symmetry; [apply inZnZ | apply inZnZ0].
+Qed.
+
+Lemma galina_fiat_crypto_p2_equiv': forall X1 X2 Y1 Y2 Z1 Z2 outx outy outz on_curve1 on_curve2 on_curveout except, 
+(BLS12_G2_add_Gallina_spec X1 Y1 Z1 X2 Y2 Z2 outx outy outz -> 
+fc_proj_p2_eq (to_fc_p2_point_from_mont outx outy outz on_curveout) (fc_proj_p2_add (to_fc_p2_point_from_mont X1 Y1 Z1 on_curve1) (to_fc_p2_point_from_mont X2 Y2 Z2 on_curve2) except)).
+Proof. intros. apply fc_proj_p2_eq_sig. rewrite (galina_fiat_crypto_p2_equiv _ _ _ _ _ _ _ _ _ on_curve1 on_curve2 except) in H.
+ unfold to_fc_p2_point_from_mont, to_fc_p2_point, proj1_sig.
+ apply pair_equal_spec in H; destruct H as [H ->]; apply pair_equal_spec in H; destruct H as [-> ->].
+ do 3 rewrite p2_backandforth. reflexivity. 
+Qed.
+
+Definition pair_valp2 x := let '(x, y, z) := x in (valp2 x, valp2 y, valp2 z).
+
+Definition encodemodp2 x := (encodemod (fst x), encodemod (snd x)).
+
+Lemma eval_encodemod_valp2 : forall v, evfrom_pair (encodemodp2 (valp2 v)) = (valp2 v).
+Proof. intros []. apply pair_equal_spec. unfold encodemodp2, valp2, fst, snd. split; apply eval_encodemod_val.  
+Qed. 
+
+Definition galina_G2_spec_from_fc_point (p1 p2 pout : fc_proj_p2_point) := 
+    let '(x1, y1, z1) := pair_valp2 (proj1_sig p1) in
+    let '(x2, y2, z2) := pair_valp2 (proj1_sig p2) in
+    let '(outx, outy, outz) := pair_valp2 (proj1_sig pout) in
+    let x1 := encodemodp2 x1 in
+    let x2 := encodemodp2 x2 in
+    let y1 := encodemodp2 y1 in
+    let y2 := encodemodp2 y2 in
+    let z1 := encodemodp2 z1 in
+    let z2 := encodemodp2 z2 in
+    let outx := encodemodp2 outx in
+    let outy := encodemodp2 outy in
+    let outz := encodemodp2 outz in
+    BLS12_G2_add_Gallina_spec x1 y1 z1 x2 y2 z2 outx outy outz.
+
+Lemma galina_fiat_crypto_p2_equiv'' : forall p1 p2 pout except,
+    fc_proj_p2_eq pout (fc_proj_p2_add p1 p2 except) ->
+    exists pout', fc_proj_p2_eq pout pout' /\ galina_G2_spec_from_fc_point p1 p2 pout'.
+Proof. intros. exists (fc_proj_p2_add p1 p2 except).
+    split; [apply H|]. unfold galina_G2_spec_from_fc_point, BLS12_G2_add_Gallina_spec, MontgomeryCurveSpecs.BLS12_G2_add_Gallina_spec.
+    destruct p1 as [[[]]]. destruct p2 as [[[]]]. unfold fc_proj_p2_add, proj1_sig, pair_valp2. 
+    repeat rewrite eval_encodemod_valp2. znz2_to_z2_arith. reflexivity.
+Qed.
